heap_lang/lib/barrier/barrier.v
@@ -1,7 +1,7 @@
 From iris.heap_lang Require Export notation.
 
 Definition newbarrier : val := λ: <>, ref #0.
-Definition signal : val := λ: "x", '"x" <- #1.
+Definition signal : val := λ: "x", "x" <- #1.
 Definition wait : val :=
-  rec: "wait" "x" := if: !'"x" = #1 then #() else '"wait" '"x".
+  rec: "wait" "x" := if: !"x" = #1 then #() else "wait" "x".
 Global Opaque newbarrier signal wait.
