heap_lang/lib/lock.v
@@ -6,8 +6,8 @@ Import uPred.
 Definition newlock : val := λ: <>, ref #false.
 Definition acquire : val :=
   rec: "acquire" "l" :=
-    if: CAS '"l" #false #true then #() else '"acquire" '"l".
-Definition release : val := λ: "l", '"l" <- #false.
+    if: CAS "l" #false #true then #() else "acquire" "l".
+Definition release : val := λ: "l", "l" <- #false.
 Global Opaque newlock acquire release.
 
 (** The CMRA we need. *)
